LeanStatefulAoc.lean
@@ -8,6 +8,7 @@ import LeanStatefulAoc.EvalMono
 import LeanStatefulAoc.EvalHMono
 import LeanStatefulAoc.EvalTripos
 import LeanStatefulAoc.EvalTopos
+import LeanStatefulAoc.EvalMemo
 import LeanStatefulAoc.FwdClosed
 import LeanStatefulAoc.Tripos
 import LeanStatefulAoc.Computation
